## Gibbs sampling

### Basic idea

$$p(\theta, \phi|y) \propto g(\theta, \phi)$$

$$p(\theta, \phi|y) = p(\phi |y)p(\theta| \phi,y)$$


__Notes__

(1) $p(\theta| \phi,y)$ is called the full conditional for theta. 

(2) We can update one parameter at a time. 


$$p(\theta| \phi,y) \propto p(\theta, \phi|y) \propto g(\theta, \phi)$$

$$p(\phi| \theta,y) \propto p(\theta, \phi|y) \propto g(\theta, \phi)$$


### Procedure

(1) Initialize $\theta_0$, $\phi_0$.

(2) For $i=1,..., m$, repeat:

     (a) Using $\phi_{i-1}$, draw $\theta_i \sim p(\theta|\phi_{i-1},y)$
     (b) Using $\theta_i$, draw $\phi_i \sim p(\phi|\theta_i,y)$
     
### Example

$$y_i|\mu, \sigma^2 \sim N(\mu, \sigma^2),i = 1, ...,n$$

$$\mu \sim N(\mu_0,\sigma_0^2)$$

$$\sigma^2 \sim IG(v_0,\beta_0)$$

$$\begin{aligned} p(\mu, \sigma^2) &\propto p(y1,...,y_n| \mu, \sigma^2)p(\mu)p(\sigma^2) \\ &=\prod_{i=1}^n[N(y_i|\mu,\sigma^2)]N(\mu|\mu_0,\sigma_0^2)IG(\sigma^2|v_0,\beta_0)\\ &= \prod_{i=1}^n [\frac{1}{\sqrt{2\pi \sigma^2}} exp(-\frac{1}{2\sigma^2}(y_i-\mu)^2)] \cdot \frac{1}{\sqrt{2\pi \sigma_0^2}} exp(-\frac{1}{2\sigma_0^2}(\mu-\mu_0)^2) \\ &\cdot \frac{\beta_0^{v_0}}{\Gamma(v_0)}(\sigma^2)^{-(v_0+1)}exp(-\frac{\beta_0}{\sigma^2}) \\ &\propto (\sigma^2)^{-\frac{n}{2}}exp[-\frac{1}{2\sigma^2} \sum_{i=1}^n(y_i-\mu)^2] \cdot exp[-\frac{1}{2\sigma_0^2}(\mu-\mu_0)^2] \cdot (\sigma^2)^{-(v_0+1)}exp[-\frac{\beta_0}{\sigma^2}] \end{aligned}$$ 


The following the full conditoinal distribution:

$$\begin{aligned} p(\mu| \sigma^2, y_1,...,y_n) &\propto p(\mu,\sigma^2 | y_1,...,y_n)\\ &\propto  exp(-\frac{1}{2\sigma^2}(y_i-\mu)^2) exp[-\frac{1}{2\sigma_0^2}(\mu-\mu_0)^2] \\ &=exp[-\frac{1}{2\sigma^2}(y_i-\mu)^2-\frac{1}{2\sigma_0^2}(\mu-\mu_0)^2] \\ &\propto N(\mu |\frac{n\bar{y}/\sigma^2+\mu_0/\sigma^2}{n/\sigma^2+1/\sigma_0^2},\frac{1}{n/\sigma^2+1/\sigma_0^2})\end{aligned}$$



$$\begin{aligned} p(\sigma^2| \mu, y_1,...,y_n) &\propto p(\mu,\sigma^2 | y_1,...,y_n)\\ &\propto  (\sigma^2)^{-\frac{n}{2}} exp(-\frac{1}{2\sigma^2}(y_i-\mu)^2) \cdot (\sigma^2)^{-(v_0+1)}exp[-\frac{\beta_0}{\sigma^2}]\\ &= (\sigma^2)^{-(v_0+\frac{n}{2}+1)}exp[-\frac{1}{\sigma^2}(\beta_0+\frac{\sum_{i=1}^n(y_i-\mu)^2}{2})] \\ &\propto IG(\sigma^2|v_0+\frac{n}{2},\beta_0+\frac{\sum_{i=1}^n(y_i-\mu)^2}{2})\end{aligned}$$


### R code

The following R code first will impletement the following for $\mu$ and $\sigma^2$ discussed above:

$$p(\mu| \sigma^2, y_1,...,y_n) \propto  N(\mu |\frac{n\bar{y}/\sigma^2+\mu_0/\sigma^2}{n/\sigma^2+1/\sigma_0^2},\frac{1}{n/\sigma^2+1/\sigma_0^2}) $$
$$ p(\sigma^2| \mu, y_1,...,y_n)  \propto IG(\sigma^2|v_0+\frac{n}{2},\beta_0+\frac{\sum_{i=1}^n(y_i-\mu)^2}{2})$$


```{R}

update_mu<-function(n,ybar, sig2,mu_0,sig2_0)
          {sig2_1=1/(n/sig2+1/sig2_0)
           mu_1=sig2_1*(n*ybar/sig2+mu_0/sig2_0)
           rnorm(n=1,mean=mu_1,sd=sqrt(sig2_1))}



update_sig2<-function(n,y,mu,nu_0,beta_0)
         {nu_1=nu_0+n/2
         sumsq=sum((y-mu)^2)
         beta_1=beta_0+sumsq/2
         out_gamma=rgamma(n=1,shape =nu_1,rate=beta_1)
         1/out_gamma}



gibbs<-function(y,n_iter,init,prior)
{
  ybar=mean(y)
  n=length(y)
  
  mu_out=numeric(n_iter)
  sig2_out=numeric(n_iter)
  
  mu_now=init$mu
  
  ## Gibbs sampler
  for (i in 1:n_iter)
  {
    sig2_now=update_sig2(n=n,y=y,mu=mu_now,nu_0 = prior$nu_0,beta_0 = prior$beta_0)
    mu_now=update_mu(n=n,ybar=ybar, sig2 = sig2_now,mu_0 = prior$mu_0,sig2_0 = prior$sig2_0)
    
    sig2_out[i]=sig2_now
    mu_out[i]=mu_now
  }
  cbind(mu=mu_out,sig2=sig2_out)
}

y=c(1.2,1.4,-0.5,0.3,0.9,2.3,1.0,0.1,1.3,1.9)
ybar=mean(y)
n=length(y)

prior=list()
prior$mu_0=0
prior$sig2_0=1

prior$n_0=2
prior$s2_0=1
prior$nu_0=prior$n_0/2
prior$beta_0=prior$n_0*prior$s2_0/2

hist(y,freq = FALSE,xlim=c(-3,3))
curve(dnorm(x=x,mean=prior$mu_0,sd=sqrt(prior$sig2_0)),lty=2,add=TRUE)
points(y,rep(0,n),pch=1)
points(ybar,0,pch=19)

set.seed(53)
init=list()
init$mu=0

post=gibbs(y=y,n_iter = 1e3,init=init,prior=prior)
head(post)
tail(post)

library(coda)
plot(as.mcmc(post))
summary(as.mcmc(post))

  
```